Cleanup & notation

ISL.v
@@ -1,199 +1,11 @@
 From iris.bi Require Import bi.
 Require Export lang.
 
-(* now that we have the starting point of our operational semantic
-   I can focus on what it means for an expression to be an error.
-   All our examples are syntactically correct (or should be) and
-   the types check out so we are referring to be _semantically
-   correct_ (?). The usage of resources in our program is correct
-   if we can always reduce an expression to a value so any
-   expression that does not reduce to a value will contain
-   a resource error or an **error** form.
- *)
-
-Definition is_val e :=
-  match e with
-  | EVal _ => true
-  | _ => false
-  end.
-
-(* our expression is an error when we cannot step anymore in the reduction *)
-Definition is_error e h := not (is_val e) ∧ ∀ e' h', not (step e h e' h').
-
-(* to unify the two definitions of wp/ewp later on we rely on this new predicate *)
-Definition is_error_or_val (v : option val) (e : expr) (m : mem): Prop :=
-  match v with
-  | None => is_error e m
-  | Some v => e = EVal v
-end.
-
-(* is_error relies on _step_ to say that an expression does not step
-   but we only have an operational semantic for not stepping that works
-   on head_step instead.
-
-   This section is about lifting this idea of non stepping to expressions
-   reducing in contexes.
-*)
-
-Lemma head_step_fill_item_val a e e' h h' :
-  head_step (fill_item a e) h e' h' → is_val e.
-Proof.
-  destruct a; simpl; intros H; inversion H; done.
-Qed.
-
-Lemma fill_item_eq_val a1 a2 e1 e2 :
-  fill_item a1 e1 = fill_item a2 e2 →
-  e1 = e2 ∨ is_val e1 ∨ is_val e2.
-Proof.
-  destruct a1,a2; simpl; intro; simplify_eq; eauto.
-Qed.
-
-Lemma head_step_not_val e1 e2 h1 h2 :
-  head_step e1 e2 h1 h2 → is_val e1 → False.
-Proof.
-  intros Hs?. by inversion Hs; subst.
-Qed.
-
-Lemma is_val_fill e E :
-  is_val (fill E e) → is_val e.
-Proof.
-  destruct E; eauto. by destruct c.
-Qed.
-
-Lemma fill_item_not_val e a :
-  ¬ is_val (fill_item a e).
-Proof.
-  destruct a; eauto.
-Qed.
-
-Lemma is_error_fill_item e h a :
-  is_error e h → is_error (fill_item a e) h.
-Proof.
-  intros [Hv Hs].
-  split; eauto using fill_item_not_val.
-  intros e' h' H. inversion H. clear H. subst.
-  induction E; simpl in *. subst.
-  - eauto using head_step_fill_item_val.
-  - apply fill_item_eq_val in H0 as [|[]];
-    eauto using is_val_fill, head_step_not_val.
-    subst. eapply Hs. constructor. done.
-Qed.
-
-Lemma is_error_fill e h E :
-  is_error e h → is_error (fill E e) h.
-Proof.
-  induction E; simpl; eauto using is_error_fill_item.
-Qed.
-
-(* finally we can now start messing around with our definitions
-   and prove that some expressions will error *)
-
-Example simple_error := is_error EError ∅.
-
-Lemma our_first_error : simple_error.
-Proof.
-  unfold simple_error.
-  split.
-  - auto.
-  - intros.
-    unfold not.
-    intro.
-    (* now we got a proof of head_step for an expression EError
-       which is not a thing in our operational semantic; the contradiction
-       must come from there.
-     *)
-    inversion H.
-    (* the inversion left us with an _unknown_ context E to work with
-       but we still have the restriction that fill E e1 = EError; this
-       only makes sense when E = [] and e1 = EError *)
-    destruct E.
-    * simpl in *; subst; inversion H1.
-    * destruct c; simpl in *; discriminate.
-Qed.
-
-(* and we can get errors also from using resources wrongly *)
-
-Lemma resource_error l: is_error (EFree (EVal (VLoc l))) ∅.
-Proof.
-  split; [auto|].
-  intros ???H.
-  erewrite step_free_inv in H.
-  destruct H as (v & _ & lookup & _).
-  rewrite lookup_empty in lookup.
-  discriminate.
-Qed.
-
-(* Now that we have found what it means for an expression to be an error
-   we can move on to whole programs that contain an error.
-
-   An expression may reduce to many values and it's not just non determinism
-   but control structures such _if_ and _while_. The idea we are after is that
-   we need to prove something may error and we encode it as _there is one reduction
-   path leading us to an error_.
-
-   The alternative is that forall paths there is no error so we can now
-   also describe correctness.
- *)
-Definition contains_error e h := ∃ e' h', steps e h e' h' ∧ is_error e' h'.
-
-(* the EAmb expression will only give us natural values but we are gonna use it
-   to express non determinism by reducing in IfCtx
-*)
-Definition amb_bool := (EOp EqOp EAmb (EVal (VNat 0))).
-
-(* and finally prove that we can always get any two booleans *)
-Lemma amb_is_ambiguous (b : bool) (m : mem) : steps amb_bool m (EVal (VBool b)) m.
-Proof.
-  unfold amb_bool.
-  eapply steps_step.
-  rewrite <- fill_op_l.
-  constructor.
-  apply (Amb_headstep m (if b then 0 else 1)).
-  rewrite fill_op_l.
-  apply steps_single.
-  destruct b; eauto using head_step.
-Qed.
-
-(* if an error state is reachable in a sub-expression then we might get lucky *)
-Lemma contains_error_mono e e' h h' :
-  steps e h e' h' → contains_error e' h' → contains_error e h.
-Proof.
-  intros.
-  unfold contains_error in *.
-  destruct H0. destruct H0. destruct H0.
-  eexists x, x0.
-  split; auto.
-  eapply steps_trans; eassumption.
-Qed.
-
-Definition will_error (P : mem → Prop) (e : expr) := ∃ h h' e', P h ∧ steps e h e' h' ∧ is_error e' h'.
-
-(* Notation "[[ P ]] e [[error]]" := (will_error P e). *)
-
-Definition reaches (P : mem → Prop) (e : expr) (Q : val → mem → Prop) :=
-  ∀ v h', Q v h' → ∃ h, P h ∧ steps e h (EVal v) h'.
-
-Notation "[ P ] e [[ v , Q ]]" := (reaches P e (fun v => Q)).
-
-Definition iEmpty (m : mem) := empty = m.
-
-Example b := ([ iEmpty ] amb_bool [[ x , iEmpty ]]).
-
-Definition under_approximation (P : mem → Prop) (e : expr) (Q : val → mem → Prop) :=
-  will_error P e ∨ reaches P e Q.
+Delimit Scope S with S.
 
 Definition iProp := mem → Prop.
 
-(* m' satisfies this predicate only if there exists m ∈ P such that m' is reachable while executing
-   program e starting from m.
-
-   As a program might error we encode this choice with the optional end value v; Some v encodes
-   that the computation ended with value v while None encodes the fact that we are stuck in an
-   error. *)
-Definition post (e : expr) (P : iProp) (v : option val) : iProp :=
-  λ m', ∀ mf, m' ##ₘ mf → (∃ m e', m ##ₘ mf ∧ P m ∧ steps e (m ∪ mf) e' (m' ∪ mf) ∧ is_error_or_val v e' (m' ∪ mf)).
-
-
+Definition iEntails (P Q : iProp) : Prop := ∀ m, P m → Q m.
 Definition iEmp : iProp := λ m, m = ∅.
 Definition iPoints (l : nat) (v : val) : iProp := λ m, m = {[ l := (Value v) ]}.
 Definition iUnallocated (l : nat) : iProp := λ m, m !! l = None.
@@ -205,529 +17,521 @@ Definition iOr (P Q : iProp) : iProp := λ m, P m ∨ Q m.
 Definition iForall {A} (P : A → iProp) : iProp := λ m, ∀ x, P x m.
 Definition iExists {A} (P : A → iProp) : iProp := λ m, ∃ x, P x m.
 Definition iPure (φ : Prop) : iProp := λ m, φ ∧ m = ∅.
-Definition iEntails (P Q : iProp) : Prop := ∀ m, P m → Q m.
 Definition iOwn (m : mem) : iProp := λ m', m' = m.
 
-Notation "P ⊢ Q" := (iEntails P Q) (at level 99, Q at level 200).
-Notation "P ∗ Q" := (iSep P Q) (at level 80, right associativity).
-Notation "P ∧_ Q" := (iAnd P Q) (at level 80, right associativity).
-Notation "P ∨_ Q" := (iOr P Q) (at level 85, right associativity).
-Notation "l ↦ v" := (iPoints l v) (at level 20).
-Notation "l ↦ ⊥" := (iNegPoints l) (at level 20).
-Notation "'emp'" := iEmp.
-Notation "P -∗ Q" := (iWand P Q) (at level 99, Q at level 200, right associativity).
-Notation "⌜ p ⌝" := (iPure p) (at level 1, p at level 200).
-Notation "'All' x1 .. xn , P" :=
-  (iForall (fun x1 => .. (iForall (fun xn => P)) ..))
-  (at level 200, x1 binder, xn binder, right associativity).
-Notation "'Ex' x1 .. xn , P" :=
-  (iExists (fun x1 => .. (iExists (fun xn => P)) ..))
-  (at level 200, x1 binder, xn binder, right associativity).
-
+Notation "P ⊢ Q" := (iEntails P%S Q%S) (at level 99, Q at level 200).
+Notation "P ∗ Q" := (iSep P%S Q%S) (at level 80, right associativity) : S.
+Notation "P ∧ Q" := (iAnd P%S Q%S) (at level 80, right associativity) : S.
+Notation "P ∨ Q" := (iOr P%S Q%S) (at level 85, right associativity) : S.
+Notation "l ↦ v" := (iPoints l v) (at level 20) : S.
+Notation "l ↦ ⊥" := (iNegPoints l) (at level 20) : S.
+Notation "'emp'" := iEmp : S.
+Notation "P -∗ Q" := (iWand P%S Q%S) (at level 99, Q at level 200, right associativity) : S.
+Notation "⌜ p ⌝" := (iPure p) (at level 1, p at level 200) : S.
+Notation "∀ x1 .. xn , P" :=
+  (iForall (fun x1 => .. (iForall (fun xn => P%S)) ..))
+  (at level 200, x1 binder, xn binder, right associativity) : S.
+Notation "∃ x1 .. xn , P" :=
+  (iExists (fun x1 => .. (iExists (fun xn => P%S)) ..))
+  (at level 200, x1 binder, xn binder, right associativity) : S.
 
 Ltac iUnfold := unfold iEmp, iNegPoints, iUnallocated, iPoints, iSep, iWand, iForall, iExists, iPure, iEntails, iAnd, iOr in *.
-Ltac duh := iUnfold;
-  naive_solver (
-    rewrite ?map_union_assoc ?left_id ?right_id;
-    simplify_map_eq;
-    try apply map_union_comm;
-    solve_map_disjoint).
 
-(* The following lemma statements are from Robbert's exercises *)
+Section seplogic.
 
-Lemma iEntails_refl P : P ⊢ P.
-Proof. duh. Qed.
+  Ltac duh := iUnfold;
+    naive_solver (
+      rewrite ?map_union_assoc ?left_id ?right_id;
+      simplify_map_eq;
+      try apply map_union_comm;
+      solve_map_disjoint).
 
-Lemma iEntails_trans P Q R : (P ⊢ Q) → (Q ⊢ R) → (P ⊢ R).
-Proof. duh. Qed.
+  (* The following lemma statements are from Robbert's exercises *)
 
-Lemma iSep_mono_l P1 P2 Q : (P1 ⊢ P2) → P1 ∗ Q ⊢ P2 ∗ Q.
-Proof. duh. Qed.
+  Lemma iEntails_refl P : P ⊢ P.
+  Proof. duh. Qed.
 
-Lemma iSep_comm P Q : P ∗ Q ⊢ Q ∗ P.
-Proof. duh. Qed.
+  Lemma iEntails_trans P Q R : (P ⊢ Q) → (Q ⊢ R) → (P ⊢ R).
+  Proof. duh. Qed.
 
-Lemma iSep_assoc P Q R : P ∗ (Q ∗ R) ⊢ (P ∗ Q) ∗ R.
-Proof. duh. Qed.
+  Lemma iSep_mono_l P1 P2 Q : (P1 ⊢ P2) → P1 ∗ Q ⊢ P2 ∗ Q.
+  Proof. duh. Qed.
 
-Lemma iSep_emp_l P : P ⊢ emp ∗ P.
-Proof. duh. Qed.
+  Lemma iSep_comm P Q : P ∗ Q ⊢ Q ∗ P.
+  Proof. duh. Qed.
 
-Lemma iSep_emp_l_inv P : emp ∗ P ⊢ P.
-Proof. duh. Qed.
+  Lemma iSep_assoc P Q R : P ∗ (Q ∗ R) ⊢ (P ∗ Q) ∗ R.
+  Proof. duh. Qed.
 
-Lemma iWand_intro_r P Q R : (P ∗ Q ⊢ R) → P ⊢ Q -∗ R.
-Proof. duh. Qed.
+  Lemma iSep_emp_l P : P ⊢ emp ∗ P.
+  Proof. duh. Qed.
 
-Lemma iWand_elim P Q : P ∗ (P -∗ Q) ⊢ Q.
-Proof. duh. Qed.
+  Lemma iSep_emp_l_inv P : emp ∗ P ⊢ P.
+  Proof. duh. Qed.
 
-Lemma iAnd_intro (P Q R : iProp) : (R ⊢ P) → (R ⊢ Q) → R ⊢ P ∧_ Q.
-Proof. duh. Qed.
+  Lemma iWand_intro_r P Q R : (P ∗ Q ⊢ R) → P ⊢ Q -∗ R.
+  Proof. duh. Qed.
 
-Lemma iAnd_elim_l (P Q : iProp) : P ∧_ Q ⊢ P.
-Proof. duh. Qed.
+  Lemma iWand_elim P Q : P ∗ (P -∗ Q) ⊢ Q.
+  Proof. duh. Qed.
 
-Lemma iAnd_elim_r (P Q : iProp) : P ∧_ Q ⊢ Q.
-Proof. duh. Qed.
+  Lemma iAnd_intro (P Q R : iProp) : (R ⊢ P) → (R ⊢ Q) → R ⊢ P ∧ Q.
+  Proof. duh. Qed.
 
-Lemma iOr_intro_l (P Q : iProp) : P ⊢ P ∨_ Q.
-Proof. duh. Qed.
+  Lemma iAnd_elim_l (P Q : iProp) : P ∧ Q ⊢ P.
+  Proof. duh. Qed.
 
-Lemma iOr_intro_r (P Q : iProp) : Q ⊢ P ∨_ Q.
-Proof. duh. Qed.
+  Lemma iAnd_elim_r (P Q : iProp) : P ∧ Q ⊢ Q.
+  Proof. duh. Qed.
 
-Lemma iOr_elim (P Q R : iProp) : (P ⊢ R) → (Q ⊢ R) → P ∨_ Q ⊢ R.
-Proof. duh. Qed.
+  Lemma iOr_intro_l (P Q : iProp) : P ⊢ P ∨ Q.
+  Proof. duh. Qed.
 
-Lemma iForall_intro {A} P (Q : A → iProp) : (∀ x, P ⊢ Q x) → (P ⊢ All x, Q x).
-Proof. duh. Qed.
+  Lemma iOr_intro_r (P Q : iProp) : Q ⊢ P ∨ Q.
+  Proof. duh. Qed.
 
-Lemma iForall_elim {A} (P : A → iProp) x : (All z, P z) ⊢ P x.
+  Lemma iOr_elim (P Q R : iProp) : (P ⊢ R) → (Q ⊢ R) → P ∨ Q ⊢ R.
+  Proof. duh. Qed.
 
-Proof. duh. Qed.
-Lemma iExists_intro {A} (P : A → iProp) x : P x ⊢ Ex z, P z.
-Proof. duh. Qed.
+  Lemma iForall_intro {A} P (Q : A → iProp) : (∀ x, P ⊢ Q x) → (P ⊢ ∀ x, Q x).
+  Proof. duh. Qed.
 
-Lemma iExists_elim {A} (P : A → iProp) Q :  (∀ x, P x ⊢ Q) → (Ex z, P z) ⊢ Q.
-Proof. duh. Qed.
+  Lemma iForall_elim {A} (P : A → iProp) x : (∀ z, P z) ⊢ P x.
 
-Lemma iSep_emp_r P : P ⊢ P ∗ emp.
-Proof. duh. Qed.
+  Proof. duh. Qed.
+  Lemma iExists_intro {A} (P : A → iProp) x : P x ⊢ ∃ z, P z.
+  Proof. duh. Qed.
 
-Lemma iSep_emp_r_inv P : P ∗ emp ⊢ P.
-Proof. duh. Qed.
+  Lemma iExists_elim {A} (P : A → iProp) Q :  (∀ x, P x ⊢ Q) → (∃ z, P z) ⊢ Q.
+  Proof. duh. Qed.
 
-Lemma iSep_mono_r P Q1 Q2 : (Q1 ⊢ Q2) → P ∗ Q1 ⊢ P ∗ Q2.
-Proof. duh. Qed.
+  Lemma iSep_emp_r P : P ⊢ P ∗ emp.
+  Proof. duh. Qed.
 
-Lemma iSep_mono P1 P2 Q1 Q2 : (P1 ⊢ P2) → (Q1 ⊢ Q2) → P1 ∗ Q1 ⊢ P2 ∗ Q2.
-Proof. duh. Qed.
+  Lemma iSep_emp_r_inv P : P ∗ emp ⊢ P.
+  Proof. duh. Qed.
 
-Lemma iSep_assoc' P Q R : (P ∗ Q) ∗ R ⊢ P ∗ (Q ∗ R).
-Proof. intros ? (? & ? & (? & ? & ?) & ?); repeat eexists; duh. Qed.
+  Lemma iSep_mono_r P Q1 Q2 : (Q1 ⊢ Q2) → P ∗ Q1 ⊢ P ∗ Q2.
+  Proof. duh. Qed.
 
-Lemma iWand_intro_l P Q R : (Q ∗ P ⊢ R) → P ⊢ Q -∗ R.
-Proof. duh. Qed.
+  Lemma iSep_mono P1 P2 Q1 Q2 : (P1 ⊢ P2) → (Q1 ⊢ Q2) → P1 ∗ Q1 ⊢ P2 ∗ Q2.
+  Proof. duh. Qed.
 
-Lemma iExist_sep {A} (P : A → iProp) Q : (Ex x, P x) ∗ Q ⊢ Ex x, P x ∗ Q.
-Proof. duh. Qed.
+  Lemma iSep_assoc' P Q R : (P ∗ Q) ∗ R ⊢ P ∗ (Q ∗ R).
+  Proof. intros ? (? & ? & (? & ? & ?) & ?); repeat eexists; duh. Qed.
 
-Lemma iPure_intro (φ : Prop) : φ → emp ⊢ ⌜ φ ⌝.
-Proof. duh. Qed.
+  Lemma iWand_intro_l P Q R : (Q ∗ P ⊢ R) → P ⊢ Q -∗ R.
+  Proof. duh. Qed.
 
-Lemma iPure_elim (φ : Prop) P Q : (φ → P ⊢ Q) → ⌜ φ ⌝ ∗ P ⊢ Q.
-Proof. duh. Qed.
+  Lemma iExist_sep {A} (P : A → iProp) Q : (∃ x, P x) ∗ Q ⊢ ∃ x, P x ∗ Q.
+  Proof. duh. Qed.
 
-Lemma iPure_elim' (φ : Prop) Q : (φ → emp ⊢ Q) → ⌜ φ ⌝ ⊢ Q.
-Proof. duh. Qed.
+  Lemma iPure_intro (φ : Prop) : φ → emp ⊢ ⌜ φ ⌝.
+  Proof. duh. Qed.
 
+  Lemma iPure_elim (φ : Prop) P Q : (φ → P ⊢ Q) → ⌜ φ ⌝ ∗ P ⊢ Q.
+  Proof. duh. Qed.
 
-(*
-  It's not very clear to me how to write those as iProps.
-  The iReaches seems plausible to me, but iError IDK.
-  Maybe will_error should just be a Prop?
-  Maybe it should have a postcondition like in the paper?
-  Maybe you can take a look at how they do a complete proof using the rules in the paper.
-  Maybe that can be used to figure out how to do it using an analogue of WP in incorrectness logic.
- *)
+  Lemma iPure_elim' (φ : Prop) Q : (φ → emp ⊢ Q) → ⌜ φ ⌝ ⊢ Q.
+  Proof. duh. Qed.
 
+End seplogic.
 
-(* as we are working in incorrectness logic there is a shift in which relation there
-   is between the presume P and the result Q of a triple.
+Section primitive_post_rules.
 
-   In incorrectness logic a triple [P]C[Q]is true when the post(C)P over approximate Q
-   while for any over approximation logic the triple {P}C{Q} is true when post(C)P is a
-   under approximation of Q.
+  Definition post (e : expr) (P : iProp) (v : option val) : iProp :=
+    λ m', ∀ mf, m' ##ₘ mf → (∃ m e', m ##ₘ mf ∧ P m ∧ steps e (m ∪ mf) e' (m' ∪ mf) ∧ is_error_or_val v e' (m' ∪ mf)).
 
-   This inversion of the _subset of_ changes the entailment order: IL triples [P]C[Q] are expressed
-   as Q ⊢ post(C)P while correctness triples {P}C{Q} are expressed as post(C)P ⊢ Q.
+  Lemma post_mono P R Q e v:
+    (P ⊢ Q) → (R ⊢ post e P v) → (R ⊢ post e Q v).
+  Proof.
+    intros ??HP????. edestruct HP; naive_solver.
+  Qed.
 
-   For IL triples then the post(C)P set over approximates the set Q and this means that
-   for any m ∈ Q there exists a m' ∈ P such that (m', m) ∈ [C].
- *)
+  Lemma post_frame P Q e v :
+    Q ∗ post e P v ⊢ post e (Q ∗ P) v.
+  Proof.
+    iUnfold.
+    intros mT (m & m' & Hq & Hwp & -> & Hdisj) mf Hdisj'.
+    edestruct (Hwp (m ∪ mf)) as (m0&e0&?&?&?&?); first solve_map_disjoint.
+    exists (m0 ∪ m), e0.
+    split_and!;[|eexists _,_;split_and!|..]; eauto;
+    try solve_map_disjoint; rewrite ?(map_union_comm m m') -?assoc_L; eauto.
+    apply map_union_comm. solve_map_disjoint.
+  Qed.
 
-(* The path from the lectures does not work as we _need_ P here (in wp)
-   and definining hoare as P ⊢ wp P e Q obviously does not make all that sense;
-   this is why we need to figure out an alternative of WP in incorrectness logic.
+  Lemma post_val v (Q : val -> iProp) :
+    (Q v) ⊢ post (EVal v) (Q v) (Some v).
+  Proof.
+    iUnfold. intros ???. repeat eexists; eauto using steps_refl.
+  Qed.
 
-   Moreover we have to show that framing here happens in the reverse direction;
-   for any frame mf in our _result_ the same frame must happen in the _assume_
-   along with the correct anti-frame.
- *)
+  Lemma post_ctxS E e P v w :
+    post (fill E (EVal w)) (post e P (Some w)) v ⊢ post (fill E e) P v.
+  Proof.
+    intros m H mf Hdisj.
+    specialize (H mf Hdisj) as (?&?&Hdisj'&H'&?&?).
+    specialize (H' mf Hdisj') as (?&?&?&?&?&?).
+    destruct v; asimpl;
+    eauto 10 using steps_trans, steps_context.
+  Qed.
 
-(* if we increase the set of initial states then we still cover all the final states *)
-Lemma post_mono P R Q e v:
-  (P ⊢ Q) → (R ⊢ post e P v) → (R ⊢ post e Q v).
-Proof.
-  intros ??HP????. edestruct HP; naive_solver.
-Qed.
-
-Lemma post_frame P Q e v :
-  Q ∗ post e P v ⊢ post e (Q ∗ P) v.
-Proof.
-  iUnfold.
-  intros mT (m & m' & Hq & Hwp & -> & Hdisj) mf Hdisj'.
-  edestruct (Hwp (m ∪ mf)) as (m0&e0&?&?&?&?); first solve_map_disjoint.
-  exists (m0 ∪ m), e0.
-  split_and!;[|eexists _,_;split_and!|..]; eauto;
-  try solve_map_disjoint; rewrite ?(map_union_comm m m') -?assoc_L; eauto.
-  apply map_union_comm. solve_map_disjoint.
-Qed.
-
-Lemma post_val v (Q : val -> iProp) :
-  (Q v) ⊢ post (EVal v) (Q v) (Some v).
-Proof.
-  iUnfold. intros ???. repeat eexists; eauto using steps_refl.
-Qed.
-
-Lemma post_ctxS E e P v w :
-  post (fill E (EVal w)) (post e P (Some w)) v ⊢ post (fill E e) P v.
-Proof.
-  intros m H mf Hdisj.
-  specialize (H mf Hdisj) as (?&?&Hdisj'&H'&?&?).
-  specialize (H' mf Hdisj') as (?&?&?&?&?&?).
-  destruct v; asimpl;
-  eauto 10 using steps_trans, steps_context.
-Qed.
-
-Lemma post_ctxN E e P:
-  post e P None ⊢ post (fill E e) P None.
-Proof.
-  intros m H mf Hdisj.
-  specialize (H mf Hdisj) as (?&?&?&?&?&?).
-  simpl. eauto 8 using steps_context, is_error_fill.
-Qed.
+  Lemma post_ctxN E e P:
+    post e P None ⊢ post (fill E e) P None.
+  Proof.
+    intros m H mf Hdisj.
+    specialize (H mf Hdisj) as (?&?&?&?&?&?).
+    simpl. eauto 8 using steps_context, is_error_fill.
+  Qed.
 
 
-Definition pure_step (e e' : expr) := ∀ h,  step e h e' h.
+  Definition pure_step (e e' : expr) := ∀ h,  step e h e' h.
 
-Lemma post_pure_step e e' P v :
-  pure_step e e' → post e' P v ⊢ post e P v.
-Proof.
-  intros pure m H mf Hdisj.
-  specialize (H mf Hdisj) as (?&?&?&?&?&?).
-  eauto 8 using steps_step.
-Qed.
+  Lemma post_pure_step e e' P v :
+    pure_step e e' → post e' P v ⊢ post e P v.
+  Proof.
+    intros pure m H mf Hdisj.
+    specialize (H mf Hdisj) as (?&?&?&?&?&?).
+    eauto 8 using steps_step.
+  Qed.
 
-Lemma post_let_step s e2 v x P:
-  post (subst s v e2) P x ⊢ post (ELet s (EVal v) e2) P x.
-Proof.
-  apply post_pure_step. intro m.
-  eauto using post_pure_step, step_single, head_step.
-Qed.
 
-Lemma post_seqS e1 e2 P w v:
-  post e2 (post e1 P (Some w)) v ⊢ post (ESeq e1 e2) P v.
-Proof.
-  intros m H.
-  rewrite <-fill_seq.
-  eapply post_ctxS.
-  simpl.
-  intros mf Hdisj.
-  destruct (H mf) as (m' &e' & H' & Hdisj' & Hsteps & Hval); auto.
-  eauto 8 with astep.
-Qed.
+  Definition no_step e := ¬ is_val e ∧ ∀ e' m m', ¬ step e m e' m'.
 
-Lemma post_seqN e1 e2 P:
-  post e1 P None ⊢ post (ESeq e1 e2) P None.
-Proof.
-  intros m H.
-  rewrite <- fill_seq.
-  apply post_ctxN.
-  assumption.
-Qed.
+  Lemma post_no_step P e :
+    no_step e -> P ⊢ post e P None.
+  Proof.
+    intros [] m Pm mf Hdisj.
+    repeat eexists; eauto using steps.
+  Qed.
 
-Lemma post_if_true t e1 e2 P v:
-  post e1 (post t P (Some (VBool true))) v ⊢ post (EIf t e1 e2) P v.
-Proof.
-  intros m H.
-  rewrite <- fill_if.
-  eapply post_ctxS.
-  simpl fill.
-  intros mf Hdisj.
-  specialize (H mf) as (m' & e' & H' & Hdisj' & Hsteps & H);
-  eauto 10 using steps_trans, steps_if_true.
-Qed.
+  Lemma no_step_EError : no_step EError.
+  Proof.
+    split; eauto using step_error.
+  Qed.
 
-Lemma post_if_false t e1 e2 P v:
-  post e2 (post t P (Some (VBool false))) v ⊢ post (EIf t e1 e2) P v.
-Proof.
-  intros m H.
-  rewrite <- fill_if.
-  eapply post_ctxS.
-  simpl fill.
-  intros mf Hdisj.
-  specialize (H mf) as (m' & e' & H' & Hdisj' & Hsteps & H);
-  eauto 10 using steps_trans, steps_if_false.
-Qed.
+  Lemma post_error P :
+    P ⊢ post EError P None.
+  Proof.
+    eapply post_no_step, no_step_EError.
+  Qed.
 
-Lemma post_while t e P v:
-  post (EIf t (ESeq e (EWhile t e)) (EVal VUnit)) P v ⊢ post (EWhile t e) P v.
-Proof.
-  iUnfold.
-  intros m H.
-  intros mf Hdisj.
-  specialize (H mf Hdisj) as (m' & e' & Hdisj' & H' & Hsteps & H).
-  eauto 8 with astep.
-Qed.
+  Lemma post_alloc1 v l :
+    l ↦ v ⊢ post (EAlloc (EVal v)) emp (Some (VLoc l)).
+  Proof.
+    iUnfold.
+    intros ?->. eexists _,_.
+    split_and!;[|done|..|done].
+    + solve_map_disjoint.
+    + rewrite left_id_L. apply step_once.
+      apply step_single.
+      rewrite -insert_union_singleton_l.
+      constructor. intros ??HH.
+      specialize (H l). revert H.
+      rewrite HH lookup_singleton //.
+  Qed.
 
-Lemma post_op op v1 v2 v P:
-  eval_bin_op op v1 v2 = Some v →
-  P ⊢ post (EOp op (EVal v1) (EVal v2)) P (Some v).
-Proof.
-  intros Hop m HP mf Hdisj.
-  repeat eexists; eauto with astep.
-Qed.
+  Lemma post_alloc2 l v:
+    l ↦ v ⊢ post (EAlloc (EVal v)) (l ↦ ⊥) (Some (VLoc l)).
+  Proof.
+    intros m H mf Hdisj.
+    exists {[ l := Reserved ]}, (EVal (VLoc l)).
+    split.
+    - (* l is not in mf so we are ok but we have to go through the disjoint definition *)
+      apply map_disjoint_spec.
+      intros.
+      unfold iPoints in H.
+      apply lookup_singleton_Some in H0 as []; asimpl.
+      assert (mf !! i = None). { solve_map_disjoint. } simplify_eq.
+    - repeat split; try done.
+      unfold iPoints in H. subst.
+      rewrite <- (insert_singleton l Reserved (Value v)).
+      apply step_once.
+      rewrite <- (insert_union_l {[l:=Reserved]} mf l (Value v)).
+      apply step_alloc.
+      unfold valid_alloc.
+      rewrite lookup_union lookup_singleton. intros.
+      destruct (mf !! l); simpl in *; simplify_eq; eauto.
+  Qed.
 
-Lemma post_amb P n :
-  P ⊢ post EAmb P (Some (VNat n)).
-Proof.
-  intros ????. eexists _,_. split_and!; simpl; eauto.
-  eauto with astep.
-Qed.
-
-Definition no_step e := ¬ is_val e ∧ ∀ e' m m', ¬ step e m e' m'.
-
-Lemma post_no_step P e :
-  no_step e -> P ⊢ post e P None.
-Proof.
-  intros [] m Pm mf Hdisj.
-  repeat eexists; eauto using steps.
-Qed.
-
-Lemma no_step_EError : no_step EError.
-Proof.
-  split; eauto using step_error.
-Qed.
-
-Lemma post_error P :
-  P ⊢ post EError P None.
-Proof.
-  eapply post_no_step, no_step_EError.
-Qed.
-
-Lemma step_once e1 e2 h1 h2 :
-  step e1 h1 e2 h2 -> steps e1 h1 e2 h2.
-Proof.
-  eauto using steps_step, steps_refl.
-Qed.
-
-Lemma post_alloc1 v l :
-  l ↦ v ⊢ post (EAlloc (EVal v)) emp (Some (VLoc l)).
-Proof.
-  iUnfold.
-  intros ?->. eexists _,_.
-  split_and!;[|done|..|done].
-  + solve_map_disjoint.
-  + rewrite left_id_L. apply step_once.
-    apply step_single.
-    rewrite -insert_union_singleton_l.
-    constructor. intros ??HH.
-    specialize (H l). revert H.
-    rewrite HH lookup_singleton //.
-Qed.
-
-Lemma post_alloc2 l v:
-  l ↦ v ⊢ post (EAlloc (EVal v)) (l ↦ ⊥) (Some (VLoc l)).
-Proof.
-  intros m H mf Hdisj.
-  exists {[ l := Reserved ]}, (EVal (VLoc l)).
-  split.
-  - (* l is not in mf so we are ok but we have to go through the disjoint definition *)
-    apply map_disjoint_spec.
-    intros.
-    unfold iPoints in H.
-    apply lookup_singleton_Some in H0 as []; asimpl.
-    assert (mf !! i = None). { solve_map_disjoint. } simplify_eq.
-  - repeat split; try done.
-    unfold iPoints in H. subst.
-    rewrite <- (insert_singleton l Reserved (Value v)).
+  Lemma post_freeS l v:
+    l ↦ ⊥ ⊢ post (EFree (EVal (VLoc l))) (l ↦ v) (Some VUnit).
+  Proof.
+    intros m H mf Hdisj.
+    exists (<[ l := (Value v) ]> m), (EVal VUnit). iUnfold. subst.
+    split_and!; rewrite ?insert_singleton; simpl; try solve_map_disjoint.
     apply step_once.
-    rewrite <- (insert_union_l {[l:=Reserved]} mf l (Value v)).
-    apply step_alloc.
-    unfold valid_alloc.
-    rewrite lookup_union lookup_singleton. intros.
-    destruct (mf !! l); simpl in *; simplify_eq; eauto.
-Qed.
+    erewrite <- (insert_singleton _ _ Reserved), <-insert_union_l.
+    eapply step_free. exists v.
+    apply lookup_union_Some_l, lookup_insert.
+  Qed.
 
-Lemma post_freeS l v:
-  l ↦ ⊥ ⊢ post (EFree (EVal (VLoc l))) (l ↦ v) (Some VUnit).
-Proof.
-  intros m H mf Hdisj.
-  exists (<[ l := (Value v) ]> m), (EVal VUnit). iUnfold. subst.
-  split_and!; rewrite ?insert_singleton; simpl; try solve_map_disjoint.
-  apply step_once.
-  erewrite <- (insert_singleton _ _ Reserved), <-insert_union_l.
-  eapply step_free. exists v.
-  apply lookup_union_Some_l, lookup_insert.
-Qed.
+  Lemma post_freeN l:
+    l ↦ ⊥ ⊢ post (EFree (EVal (VLoc l))) (l ↦ ⊥) None.
+  Proof.
+    intros m H mf Hdisj.
+    eexists _,_.
+    split_and!;eauto with astep.
+    split; auto.
+    intros e' m' Hstep.
+    apply step_free_inv in Hstep as (? & ? & []). iUnfold. subst.
+    apply lookup_union_Some in H1 as []; eauto.
+    + apply lookup_singleton_Some in H as []. asimpl.
+    + specialize (Hdisj l). rewrite H in Hdisj.
+      rewrite lookup_singleton in Hdisj. by asimpl.
+  Qed.
 
-Lemma post_double_free l:
-  l ↦ ⊥ ⊢ post (EFree (EVal (VLoc l))) (l ↦ ⊥) None.
-Proof.
-  intros m H mf Hdisj.
-  eexists _,_.
-  split_and!;eauto with astep.
-  split; auto.
-  intros e' m' Hstep.
-  apply step_free_inv in Hstep as (? & ? & []). iUnfold. subst.
-  apply lookup_union_Some in H1 as []; eauto.
-  + apply lookup_singleton_Some in H as []. asimpl.
-  + specialize (Hdisj l). rewrite H in Hdisj.
-    rewrite lookup_singleton in Hdisj. by asimpl.
-Qed.
+  Lemma post_loadS l v:
+    l ↦ v ⊢ post (ELoad (EVal (VLoc l))) (l ↦ v) (Some v).
+  Proof.
+    intros m H mf Hdisj.
+    exists m, (EVal v). simpl.
+    split_and!; eauto.
+    iUnfold. subst.
+    apply step_once, step_load, lookup_union_Some_l, lookup_singleton.
+  Qed.
 
-Lemma post_loadS l v:
-  l ↦ v ⊢ post (ELoad (EVal (VLoc l))) (l ↦ v) (Some v).
-Proof.
-  intros m H mf Hdisj.
-  exists m, (EVal v). simpl.
-  split_and!; eauto.
-  iUnfold. subst.
-  apply step_once, step_load, lookup_union_Some_l, lookup_singleton.
-Qed.
+  Lemma post_loadN l:
+    iNegPoints l ⊢ post (ELoad (EVal (VLoc l))) (iNegPoints l) None.
+  Proof.
+    intros m H mf Hdisj.
+    eexists _,_.
+    split_and!; eauto with astep. simpl.
+    split; auto. iUnfold. subst.
+    intros e  m' Hstep.
+    apply step_load_inv in Hstep as ( v & ( -> & Hm & _)).
+    apply lookup_union_Some in Hm as []; auto.
+    + rewrite lookup_singleton in H. asimpl.
+    + specialize (Hdisj l). rewrite H in Hdisj.
+      rewrite lookup_singleton in Hdisj. by asimpl.
+  Qed.
 
-Lemma post_loadN l:
-  iNegPoints l ⊢ post (ELoad (EVal (VLoc l))) (iNegPoints l) None.
-Proof.
-  intros m H mf Hdisj.
-  eexists _,_.
-  split_and!; eauto with astep. simpl.
-  split; auto. iUnfold. subst.
-  intros e  m' Hstep.
-  apply step_load_inv in Hstep as ( v & ( -> & Hm & _)).
-  apply lookup_union_Some in Hm as []; auto.
-  + rewrite lookup_singleton in H. asimpl.
-  + specialize (Hdisj l). rewrite H in Hdisj.
-    rewrite lookup_singleton in Hdisj. by asimpl.
-Qed.
+  Lemma post_storeS l v v':
+    (l ↦ v') ⊢ post (EStore (EVal (VLoc l)) (EVal v')) (l ↦ v) (Some VUnit).
+  Proof.
+    intros m H mf Hdisj.
+    exists (<[ l := Value v ]> m), (EVal VUnit). iUnfold. subst.
+    rewrite !insert_singleton.
+    split_and!;simpl;eauto.
+    + solve_map_disjoint.
+    + eapply step_once. apply step_single.
+      erewrite <-(insert_singleton _ _ (Value v')), <-insert_union_l.
+      econstructor. apply lookup_union_Some_l, lookup_singleton.
+  Qed.
 
-Lemma post_storeS l v v':
-  (l ↦ v') ⊢ post (EStore (EVal (VLoc l)) (EVal v')) (l ↦ v) (Some VUnit).
-Proof.
-  intros m H mf Hdisj.
-  exists (<[ l := Value v ]> m), (EVal VUnit). iUnfold. subst.
-  rewrite !insert_singleton.
-  split_and!;simpl;eauto.
-  + solve_map_disjoint.
-  + eapply step_once. apply step_single.
-    erewrite <-(insert_singleton _ _ (Value v')), <-insert_union_l.
-    econstructor. apply lookup_union_Some_l, lookup_singleton.
-Qed.
+  Lemma post_storeN l v:
+    (l ↦ ⊥) ⊢ post (EStore (EVal (VLoc l)) (EVal v)) (l ↦ ⊥) None.
+  Proof.
+    intros m H mf Hdisj.
+    eexists _,_; split_and!; eauto with astep. simpl. iUnfold.
+    split; auto.
+    intros e' m' Hstep.
+    erewrite step_store_inv in Hstep.
+    destruct Hstep as (w & lookup_some & unit & final_heap).
+    erewrite lookup_union_Some_l in lookup_some.
+    2: { unfold iNegPoints in H. subst m. apply lookup_singleton. }
+    discriminate.
+  Qed.
 
-Lemma post_storeN l v:
-  (l ↦ ⊥) ⊢ post (EStore (EVal (VLoc l)) (EVal v)) (l ↦ ⊥) None.
-Proof.
-  intros m H mf Hdisj.
-  eexists _,_; split_and!; eauto with astep. simpl. iUnfold.
-  split; auto.
-  intros e' m' Hstep.
-  erewrite step_store_inv in Hstep.
-  destruct Hstep as (w & lookup_some & unit & final_heap).
-  erewrite lookup_union_Some_l in lookup_some.
-  2: { unfold iNegPoints in H. subst m. apply lookup_singleton. }
-  discriminate.
-Qed.
+End primitive_post_rules.
 
-(* the incorrectness triple is valid if for any state describe by (Q v)
-   we can reach it from a state in P after executing P under final value v.
 
-   Point wise entailment here represents the subset relation so (Q v) ⊂ post e P v
+Section derived_post_rules.
 
-   NB this is still correct for Q v = false as no heap satisfies false *)
-Definition hoare (P : iProp) (e : expr) (Q : val -> iProp) : Prop :=
-  ∀ v, (Q v) ⊢ (post e P (Some v)).
+  Lemma post_let_step s e2 v x P:
+    post (subst s v e2) P x ⊢ post (ELet s (EVal v) e2) P x.
+  Proof.
+    apply post_pure_step. intro m.
+    eauto using post_pure_step, step_single, head_step.
+  Qed.
 
-Definition hoare_err (P : iProp) (e : expr) (Q : iProp) : Prop :=
-  Q ⊢ (post e P None).
+  Lemma post_seqS e1 e2 P w v:
+    post e2 (post e1 P (Some w)) v ⊢ post (ESeq e1 e2) P v.
+  Proof.
+    intros m H.
+    rewrite <-fill_seq.
+    eapply post_ctxS.
+    simpl.
+    intros mf Hdisj.
+    destruct (H mf) as (m' &e' & H' & Hdisj' & Hsteps & Hval); auto.
+    eauto 8 with astep.
+  Qed.
 
-Definition hoare' (P : iProp) (e : expr) (Q : val -> iProp) : Prop :=
-  ∀ v m', Q v m' -> ∃ (m : mem) e', P m ∧ steps e m e' m' ∧ is_error_or_val (Some v) e' m'.
+  Lemma post_seqN e1 e2 P:
+    post e1 P None ⊢ post (ESeq e1 e2) P None.
+  Proof.
+    intros m H.
+    rewrite <- fill_seq.
+    apply post_ctxN.
+    assumption.
+  Qed.
 
-Lemma hoare_hoare' P e Q :
-  hoare P e Q -> hoare' P e Q.
-Proof.
-  intros H???. edestruct H as (?&?&?&?&?&?);[eauto|apply map_disjoint_empty_r|].
-  eexists _,_. rewrite !right_id_L in H3. split_and!; eauto.
-Qed.
+  Lemma post_if_true t e1 e2 P v:
+    post e1 (post t P (Some (VBool true))) v ⊢ post (EIf t e1 e2) P v.
+  Proof.
+    intros m H.
+    rewrite <- fill_if.
+    eapply post_ctxS.
+    simpl fill.
+    intros mf Hdisj.
+    specialize (H mf) as (m' & e' & H' & Hdisj' & Hsteps & H);
+    eauto 10 using steps_trans, steps_if_true.
+  Qed.
 
-Definition hoare_err' (P : iProp) (e : expr) (Q : iProp) : Prop :=
-  ∀ m', Q m' -> ∃ (m : mem) e', P m ∧ steps e m e' m' ∧ is_error_or_val None e' m'.
+  Lemma post_if_false t e1 e2 P v:
+    post e2 (post t P (Some (VBool false))) v ⊢ post (EIf t e1 e2) P v.
+  Proof.
+    intros m H.
+    rewrite <- fill_if.
+    eapply post_ctxS.
+    simpl fill.
+    intros mf Hdisj.
+    specialize (H mf) as (m' & e' & H' & Hdisj' & Hsteps & H);
+    eauto 10 using steps_trans, steps_if_false.
+  Qed.
 
-Lemma hoare_err_hoare_err' P e Q :
-  hoare_err P e Q -> hoare_err' P e Q.
-Proof.
-  intros H??. edestruct H as (?&?&?&?&?&?);[eauto|apply map_disjoint_empty_r|].
-  eexists _,_. rewrite !right_id_L in H3,H4. split_and!; eauto.
-Qed.
+  Lemma post_while t e P v:
+    post (EIf t (ESeq e (EWhile t e)) (EVal VUnit)) P v ⊢ post (EWhile t e) P v.
+  Proof.
+    iUnfold.
+    intros m H.
+    intros mf Hdisj.
+    specialize (H mf Hdisj) as (m' & e' & Hdisj' & H' & Hsteps & H).
+    eauto 8 with astep.
+  Qed.
 
-Lemma hoare_alloc1 v :
-  hoare emp (EAlloc (EVal v)) (λ r, Ex l, ⌜ r = VLoc l ⌝ ∗ l ↦ v).
-Proof.
-  intros v'.
-  eapply iExists_elim.
-  intros l.
-  eapply iPure_elim.
-  intros ->.
-  eapply post_alloc1.
-Qed.
+  Lemma post_op op v1 v2 v P:
+    eval_bin_op op v1 v2 = Some v →
+    P ⊢ post (EOp op (EVal v1) (EVal v2)) P (Some v).
+  Proof.
+    intros Hop m HP mf Hdisj.
+    repeat eexists; eauto with astep.
+  Qed.
 
-Lemma hoare_alloc2 l v :
-  hoare (l ↦ ⊥) (EAlloc (EVal v)) (λ r, ⌜ r = VLoc l ⌝ ∗ l ↦ v).
-Proof.
-  intros v'.
-  eapply iPure_elim.
-  intros ->.
-  eapply post_alloc2.
-Qed.
+  Lemma post_amb P n :
+    P ⊢ post EAmb P (Some (VNat n)).
+  Proof.
+    intros ????. eexists _,_. split_and!; simpl; eauto.
+    eauto with astep.
+  Qed.
 
-Lemma hoare_amb n :
-  hoare emp EAmb (λ v, ⌜ v = VNat n ⌝).
-Proof.
-  intros v.
-  eapply iPure_elim'.
-  intros ->.
-  eapply post_amb.
-Qed.
+End derived_post_rules.
 
-Lemma hoare_disj P1 P2 Q1 Q2 e :
-  hoare P1 e Q1 -> hoare P2 e Q2 -> hoare (P1 ∨_ P2) e (λ v, Q1 v ∨_ Q2 v).
-Proof.
-  unfold hoare.
-  intros H1 H2 v. specialize (H1 v). specialize (H2 v).
-  eapply iOr_elim.
-  + eapply post_mono. eapply iOr_intro_l. done.
-  + eapply post_mono. eapply iOr_intro_r. done.
-Qed.
+Section hoare.
 
-Lemma hoare_exists {A} (P : A -> iProp) Q e :
-  (∀ x, hoare (P x) e (λ v, Q x v)) -> hoare (Ex x, P x) e (λ v, Ex x, Q x v).
-Proof.
-  unfold hoare. eauto using post_mono, iExists_intro, iExists_elim.
-Qed.
+  (* the incorrectness triple is valid if for any state describe by (Q v)
+    we can reach it from a state in P after executing P under final value v.
 
-Lemma hoare_let : True. Proof. done. Qed.
-Lemma hoare_while : True. Proof. done. Qed.
-Lemma hoare_seqS : True. Proof. done. Qed.
-Lemma hoare_seqN : True. Proof. done. Qed.
-Lemma hoare_cons : True. Proof. done. Qed.
-Lemma hoare_error : True. Proof. done. Qed.
-Lemma hoare_frame : True. Proof. done. Qed.
-Lemma hoare_freeS : True. Proof. done. Qed.
-Lemma hoare_freeN : True. Proof. done. Qed.
-Lemma hoare_loadS : True. Proof. done. Qed.
-Lemma hoare_loadN : True. Proof. done. Qed.
-Lemma hoare_storeS : True. Proof. done. Qed.
-Lemma hoare_storeN : True. Proof. done. Qed.
-Lemma hoare_op : True. Proof. done. Qed.
-Lemma hoare_pure_step : True. Proof. done. Qed.
-Lemma hoare_val : True. Proof. done. Qed.
-Lemma hoare_ctxS : True. Proof. done. Qed.
-Lemma hoare_ctxN : True. Proof. done. Qed.
-Lemma hoare_if_true : True. Proof. done. Qed.
-Lemma hoare_if_false : True. Proof. done. Qed.
+    Point wise entailment here represents the subset relation so (Q v) ⊂ post e P v
 
+    NB this is still correct for Q v = false as no heap satisfies false *)
+  Definition hoare (P : iProp) (e : expr) (Q : val -> iProp) : Prop :=
+    ∀ v, (Q v) ⊢ (post e P (Some v)).
+
+  Definition hoare_err (P : iProp) (e : expr) (Q : iProp) : Prop :=
+    Q ⊢ (post e P None).
+
+  Notation "{{ P }} e {{ v , Q }}" := (hoare P%S e (λ v, Q%S))
+    (at level 20, e, P at level 200, Q at level 200, only parsing).
+
+  Notation "{{ P }} e {{ERR: Q }}" := (hoare_err P%S e Q%S)
+    (at level 20, e, P at level 200, Q at level 200, only parsing).
+
+
+  Definition hoare' (P : iProp) (e : expr) (Q : val -> iProp) : Prop :=
+    ∀ v m', Q v m' -> ∃ (m : mem) e', P m ∧ steps e m e' m' ∧ is_error_or_val (Some v) e' m'.
+
+  Lemma hoare_hoare' P e Q :
+    hoare P e Q -> hoare' P e Q.
+  Proof.
+    intros H???. edestruct H as (?&?&?&?&?&?);[eauto|apply map_disjoint_empty_r|].
+    eexists _,_. rewrite !right_id_L in H3. split_and!; eauto.
+  Qed.
+
+  Definition hoare_err' (P : iProp) (e : expr) (Q : iProp) : Prop :=
+    ∀ m', Q m' -> ∃ (m : mem) e', P m ∧ steps e m e' m' ∧ is_error_or_val None e' m'.
+
+  Lemma hoare_err_hoare_err' P e Q :
+    hoare_err P e Q -> hoare_err' P e Q.
+  Proof.
+    intros H??. edestruct H as (?&?&?&?&?&?);[eauto|apply map_disjoint_empty_r|].
+    eexists _,_. rewrite !right_id_L in H3,H4. split_and!; eauto.
+  Qed.
+
+  Lemma hoare_alloc1 v :
+    {{ emp }} (EAlloc (EVal v)) {{ r, ∃ l, ⌜ r = VLoc l ⌝  ∗ l ↦ v }}.
+  Proof.
+    intros v'.
+    eapply iExists_elim.
+    intros l.
+    eapply iPure_elim.
+    intros ->.
+    eapply post_alloc1.
+  Qed.
+
+  Lemma hoare_alloc2 l v :
+    {{ l ↦ ⊥ }} (EAlloc (EVal v)) {{ r, ⌜ r = VLoc l ⌝ ∗ l ↦ v }}.
+  Proof.
+    intros v'.
+    eapply iPure_elim.
+    intros ->.
+    eapply post_alloc2.
+  Qed.
+
+  Lemma hoare_amb n :
+    {{ emp }} EAmb {{ v, ⌜ v = VNat n ⌝ }}.
+  Proof.
+    intros v.
+    eapply iPure_elim'.
+    intros ->.
+    eapply post_amb.
+  Qed.
+
+  Lemma hoare_disj P1 P2 Q1 Q2 e :
+    {{ P1 }} e {{ v, Q1 v }} ->
+    {{ P2 }} e {{ v, Q2 v }} ->
+    {{ P1 ∨ P2 }} e {{ v, Q1 v ∨ Q2 v }}.
+  Proof.
+    unfold hoare.
+    intros H1 H2 v. specialize (H1 v). specialize (H2 v).
+    eapply iOr_elim.
+    + eapply post_mono. eapply iOr_intro_l. done.
+    + eapply post_mono. eapply iOr_intro_r. done.
+  Qed.
+
+  Lemma hoare_exists {A} (P : A -> iProp) Q e :
+    (∀ x, {{ (P x) }} e {{ v, Q x v }}) -> {{ ∃ x, P x }} e {{ v, ∃ x, Q x v }}.
+  Proof.
+    unfold hoare. eauto using post_mono, iExists_intro, iExists_elim.
+  Qed.
+
+  Lemma hoare_error P Q :
+    {{ P }} EError {{ERR: Q }}.
+  Proof.
+  Admitted.
+
+  Lemma hoare_let : True. Proof. done. Qed.
+  Lemma hoare_while : True. Proof. done. Qed.
+  Lemma hoare_seqS : True. Proof. done. Qed.
+  Lemma hoare_seqN : True. Proof. done. Qed.
+  Lemma hoare_cons : True. Proof. done. Qed.
+  Lemma hoare_error : True. Proof. done. Qed.
+  Lemma hoare_frame : True. Proof. done. Qed.
+  Lemma hoare_freeS : True. Proof. done. Qed.
+  Lemma hoare_freeN : True. Proof. done. Qed.
+  Lemma hoare_loadS : True. Proof. done. Qed.
+  Lemma hoare_loadN : True. Proof. done. Qed.
+  Lemma hoare_storeS : True. Proof. done. Qed.
+  Lemma hoare_storeN : True. Proof. done. Qed.
+  Lemma hoare_op : True. Proof. done. Qed.
+  Lemma hoare_pure_step : True. Proof. done. Qed.
+  Lemma hoare_val : True. Proof. done. Qed.
+  Lemma hoare_ctxS : True. Proof. done. Qed.
+  Lemma hoare_ctxN : True. Proof. done. Qed.
+  Lemma hoare_if_true : True. Proof. done. Qed.
+  Lemma hoare_if_false : True. Proof. done. Qed.
+
+End hoare.
 (* this is about evaluation of pure expressions *)
 
 (*
